pcuic/theories/PCUICCases.v
@@ -1,0 +1,235 @@
+(* Distributed under the terms of the MIT license. *)
+From MetaCoq.Template Require Import config utils.
+From MetaCoq.PCUIC Require Import PCUICAst PCUICAstUtils
+     PCUICLiftSubst PCUICEquality PCUICUnivSubst PCUICInduction.
+
+Require Import ssreflect.
+Require Import Equations.Prop.DepElim.
+From Equations.Type Require Import Relation Relation_Properties.
+From Equations Require Import Equations.
+Set Equations Transparent.
+Set Default Goal Selector "!".
+
+(** * Functions related to the "compact" case representation *)
+
+(** Inductive substitution, to produce a constructors' type *)
+Definition inds ind u (l : list one_inductive_body) :=
+  let fix aux n :=
+      match n with
+      | 0 => []
+      | S n => tInd (mkInd ind n) u :: aux n
+      end
+  in aux (List.length l).
+
+Lemma inds_length ind u l : #|inds ind u l| = #|l|.
+Proof.
+  unfold inds. induction l; simpl; congruence.
+Qed.
+Hint Rewrite inds_length : len.
+
+Lemma inds_spec ind u l :
+  inds ind u l = List.rev (mapi (fun i _ => tInd {| inductive_mind := ind; inductive_ind := i |} u) l).
+Proof.
+  unfold inds, mapi. induction l using rev_ind.
+  - simpl. reflexivity.
+  - now rewrite app_length /= Nat.add_1_r IHl mapi_rec_app /= rev_app_distr /= Nat.add_0_r.
+Qed.
+
+(** For cases typing *)
+
+Inductive instantiate_params_subst_spec : context -> list term -> list term -> term -> list term -> term -> Prop :=
+| instantiate_params_subst_nil s ty : instantiate_params_subst_spec [] [] s ty s ty
+| instantiate_params_subst_vass na ty params pari pars s na' ty' pty s' pty' : 
+  instantiate_params_subst_spec params pars (pari :: s) pty s' pty' ->
+  instantiate_params_subst_spec (vass na ty :: params) (pari :: pars) s (tProd na' ty' pty) s' pty'
+| instantiate_params_subst_vdef na b ty params pars s na' b' ty' pty s' pty' : 
+  instantiate_params_subst_spec params pars (subst s 0 b :: s) pty s' pty' ->
+  instantiate_params_subst_spec (vdef na b ty :: params) pars s (tLetIn na' b' ty' pty) s' pty'.
+Derive Signature for instantiate_params_subst_spec.
+
+
+(** Compute the type of a case from the predicate [p], actual parameters [pars] and
+    an inductive declaration. *)
+
+Fixpoint instantiate_params_subst
+         (params : context)
+         (pars s : list term)
+         (ty : term) : option (list term × term) :=
+  match params with
+  | [] => match pars with
+          | [] => Some (s, ty)
+          | _ :: _ => None (* Too many arguments to substitute *)
+          end
+  | d :: params =>
+    match d.(decl_body), ty with
+    | None, tProd _ _ B =>
+      match pars with
+      | hd :: tl => instantiate_params_subst params tl (hd :: s) B
+      | [] => None (* Not enough arguments to substitute *)
+      end
+    | Some b, tLetIn _ _ _ b' => instantiate_params_subst params pars (subst0 s b :: s) b'
+    | _, _ => None (* Not enough products in the type *)
+    end
+  end.
+
+Lemma instantiate_params_substP params pars s ty s' ty' : 
+  instantiate_params_subst params pars s ty = Some (s', ty') <->
+  instantiate_params_subst_spec params pars s ty s' ty'.
+Proof.
+  induction params in pars, s, ty |- *.
+  - split.
+    * destruct pars => /= // => [= -> ->].
+      constructor.
+    * intros. depelim H. reflexivity.
+  - split.
+    * destruct a as [na [b|] ?] => /=; destruct ty => //.
+      + move/IHparams.
+        intros. now constructor.
+      + destruct pars => //.
+        move/IHparams.
+        now constructor.
+    * intros H; depelim H; simpl;
+      now apply IHparams.
+Qed.
+
+
+Fixpoint map2 {A B C} (f : A -> B -> C) (l : list A) (l' : list B) : list C :=
+  match l, l' with
+  | hd :: tl, hd' :: tl' => f hd hd' :: map2 f tl tl'
+  | _, _ => []
+  end.
+
+Definition set_binder_name (na : aname) (x : context_decl) : context_decl :=
+  {| decl_name := na;
+     decl_body := decl_body x;
+     decl_type := decl_type x |}.
+
+Universe cpred.
+
+Variant ind_case_predicate_context ind mdecl idecl params puinst pctx : context -> Type@{cpred} :=
+| mk_ind_case_predicate_context s ty ictx inds : 
+  instantiate_params_subst_spec 
+    (List.rev (subst_instance_context puinst (ind_params mdecl))) params []
+    (subst_instance_constr puinst (ind_type idecl)) s ty ->
+  let sty := subst s 0 ty in
+  sty = it_mkProd_or_LetIn ictx (tSort inds) ->
+  #|pctx| = S #|ictx| ->
+  let indty := mkApps (tInd ind puinst) (map (lift0 #|ictx|) params ++ to_extended_list ictx) in
+  let inddecl := 
+    {| decl_name := 
+      {| binder_name := nNamed (ind_name idecl) ;
+         binder_relevance := idecl.(ind_relevance) |};
+       decl_body := None;
+       decl_type := indty |}
+  in
+  let ictx' := map2 (fun na decl => set_binder_name na decl) pctx ictx in
+  ind_case_predicate_context ind mdecl idecl params puinst pctx ictx'.
+
+Variant case_predicate_context Σ ci p : context -> Type@{cpred} :=
+| mk_case_predicate_context mdecl idecl pctx :
+  declared_inductive Σ mdecl (ci_ind ci) idecl ->
+  ind_case_predicate_context (ci_ind ci) mdecl idecl p.(pparams) p.(puinst) p.(pcontext) pctx ->
+  case_predicate_context Σ ci p pctx.
+  
+Variant ind_case_branch_context ind mdecl (cdecl : ident * term * nat) p : context -> Type@{cpred} :=
+| mk_ind_case_branch_context s ty argctx indices : 
+    instantiate_params_subst_spec (List.rev (subst_instance_context p.(puinst) (ind_params mdecl))) p.(pparams) []
+      (subst_instance_constr p.(puinst) (cdecl.1.2)) s ty ->
+    let sty := subst s 0 ty in
+    sty = it_mkProd_or_LetIn argctx (mkApps (tInd ind p.(puinst)) (map (lift0 #|argctx|) p.(pparams) ++ indices)) ->
+    ind_case_branch_context ind mdecl cdecl p argctx.
+
+Definition ind_case_branches_contexts ind mdecl idecl p : list context -> Type@{cpred} :=
+  All2 (fun cdecl brctx => ind_case_branch_context ind mdecl cdecl p brctx) idecl.(ind_ctors).
+
+Variant case_branches_contexts Σ ci p : list context -> Type@{cpred} :=
+  | mk_case_branches_contexts mdecl idecl brsctx : 
+    declared_inductive Σ mdecl (ci_ind ci) idecl ->
+    ind_case_branches_contexts (ci_ind ci) mdecl idecl p brsctx ->
+    case_branches_contexts Σ ci p brsctx.
+
+Variant ind_case_branch_type ind mdecl (cdecl : ident * term * nat) i p pctx : context -> term -> Type@{cpred} :=
+| mk_ind_case_branch_type s ty argctx indices : 
+  instantiate_params_subst_spec (List.rev (subst_instance_context p.(puinst) (ind_params mdecl))) p.(pparams) []
+    (subst_instance_constr p.(puinst) (cdecl.1.2)) s ty ->
+  let sty := subst s 0 ty in
+  sty = it_mkProd_or_LetIn argctx (mkApps (tInd ind p.(puinst)) (map (lift0 #|argctx|) p.(pparams) ++ indices)) ->
+  let cstr := tConstruct ind i p.(puinst) in
+  let args := to_extended_list argctx in
+  let cstrapp := mkApps cstr (map (lift0 #|argctx|) p.(pparams) ++ args) in
+  let ptm := it_mkLambda_or_LetIn pctx p.(preturn) in
+  let ty := mkApps (lift0 #|argctx| ptm) (indices ++ [cstrapp]) in
+  ind_case_branch_type ind mdecl cdecl i p pctx argctx ty.
+
+Definition ind_case_branches_types ind mdecl idecl p pctx : list (context * term) -> Type@{cpred} :=
+  All2i (fun i cdecl '(brctx, brty) => ind_case_branch_type ind mdecl cdecl i p pctx brctx brty) 0 idecl.(ind_ctors).
+
+
+(* If [ty] is [Π params . B] *)
+(* and [⊢ pars : params] *)
+(* then [instantiate_params] is [B{pars}] *)
+Definition instantiate_params (params : context) (pars : list term) (ty : term) : option term :=
+  match instantiate_params_subst (List.rev params) pars [] ty with
+  | Some (s, ty) => Some (subst0 s ty)
+  | None => None
+  end.
+    
+Lemma instantiate_params_ params pars ty :
+  instantiate_params params pars ty
+  = option_map (fun '(s, ty) => subst0 s ty)
+               (instantiate_params_subst (List.rev params) pars [] ty).
+Proof.
+  unfold instantiate_params.
+  repeat (destruct ?; cbnr).
+Qed.
+(* 
+(* [params], [p] and output are already instanciated by [u] *)
+Definition build_branches_type ind mdecl idecl params u p : list (option (nat × term)) :=
+  let inds := inds ind.(inductive_mind) u mdecl.(ind_bodies) in
+  let branch_type i '(id, t, ar) :=
+    let ty := subst0 inds (subst_instance_constr u t) in
+    match instantiate_params (subst_instance_context u mdecl.(ind_params)) params ty with
+    | Some ty =>
+      let '(sign, ccl) := decompose_prod_assum [] ty in
+      let nargs := List.length sign in
+      let allargs := snd (decompose_app ccl) in
+      let '(paramrels, args) := chop mdecl.(ind_npars) allargs in
+      let cstr := tConstruct ind i u in
+      let args := (args ++ [mkApps cstr (paramrels ++ to_extended_list sign)]) in
+      Some (ar, it_mkProd_or_LetIn sign (mkApps (lift0 nargs p) args))
+    | None => None
+    end
+  in mapi branch_type idecl.(ind_ctors).
+
+Lemma build_branches_type_ ind mdecl idecl params u p :
+  build_branches_type ind mdecl idecl params u p
+  = let inds := inds ind.(inductive_mind) u mdecl.(ind_bodies) in
+    let branch_type i '(id, t, ar) :=
+        let ty := subst0 inds (subst_instance_constr u t) in
+        option_map (fun ty =>
+         let '(sign, ccl) := decompose_prod_assum [] ty in
+         let nargs := List.length sign in
+         let allargs := snd (decompose_app ccl) in
+         let '(paramrels, args) := chop mdecl.(ind_npars) allargs in
+         let cstr := tConstruct ind i u in
+         let args := (args ++ [mkApps cstr (paramrels ++ to_extended_list sign)]) in
+         (ar, it_mkProd_or_LetIn sign (mkApps (lift0 nargs p) args)))
+                  (instantiate_params (subst_instance_context u mdecl.(ind_params))
+                                      params ty)
+    in mapi branch_type idecl.(ind_ctors).
+Proof.
+  apply mapi_ext. intros ? [[? ?] ?]; cbnr.
+  repeat (destruct ?; cbnr).
+Qed. *)
+
+
+(* [params] and output already instantiated by [u] *)
+Definition build_case_predicate_context ind mdecl idecl params u : option context :=
+  index_part <- instantiate_params (subst_instance_context u (ind_params mdecl)) params
+                                   (subst_instance_constr u (ind_type idecl)) ;;
+  '(Γ, _) <- destArity [] index_part ;;
+  let inddecl :=
+      {| decl_name := mkBindAnn (nNamed idecl.(ind_name)) idecl.(ind_relevance);
+         decl_body := None;
+         decl_type := mkApps (tInd ind u) (map (lift0 #|Γ|) params ++ to_extended_list Γ) |} in
+  ret (Γ,, inddecl).
